Incremental/SalsaC.lean
@@ -1,10 +1,33 @@
 module
 
-public import Incremental.Salsa
+public import Incremental.Basic
+
+@[expose] public section
 
 namespace Incremental
 
 open Std (DHashMap HashMap)
+
+namespace SalsaC
+
+structure Memo (ℭ : BuildConfig) (q : ℭ.Q) where
+  value : ℭ.R q
+  changedAt : Nat
+  verifiedAt : Nat
+  queryDeps : Array (QueryDep ℭ q)
+  inputDeps : Array (InputDep ℭ.I)
+  hash : UInt64
+
+abbrev Memos (ℭ : BuildConfig) [BEq ℭ.Q] [Hashable ℭ.Q] := DHashMap ℭ.Q (Memo ℭ)
+
+structure Store (ℭ : BuildConfig) [BEq ℭ.I] [Hashable ℭ.I] [BEq ℭ.Q] [Hashable ℭ.Q]
+    (J : Type) where
+  inputs : J
+  revision : Nat
+  memos : Memos ℭ
+  inputRevisions : HashMap ℭ.I Nat
+
+end SalsaC
 
 variable
   (ℭ : BuildConfig)
@@ -12,7 +35,7 @@ variable
   [BEq ℭ.I] [LawfulBEq ℭ.I] [Hashable ℭ.I]
   [BEq ℭ.Q] [LawfulBEq ℭ.Q] [Hashable ℭ.Q] [∀ q, Hashable (ℭ.R q)]
 
-instance : Inhabited (Tasks ℭ → ∀ q, Salsa.Store ℭ J → ℭ.R q × Salsa.Store ℭ J) where
+instance : Inhabited (Tasks ℭ → ∀ q, SalsaC.Store ℭ J → ℭ.R q × SalsaC.Store ℭ J) where
   default tasks q s := ⟨compute tasks (Input.get s.inputs) q, s⟩
 
 @[extern "lean_salsa_build"]
@@ -22,11 +45,11 @@ public opaque salsaCBuild
     [BEq ℭ.Q] [Hashable ℭ.Q] [∀ q, Hashable (ℭ.R q)]
     [Input ℭ J] :
     Tasks ℭ → ∀ q,
-    Salsa.Store ℭ J → ℭ.R q × Salsa.Store ℭ J
+    SalsaC.Store ℭ J → ℭ.R q × SalsaC.Store ℭ J
 
 set_option warn.sorry false in
 @[expose] public def SalsaC (tasks : Tasks ℭ) : Build ℭ J tasks Id Id where
-  σ := Salsa.Store ℭ J
+  σ := SalsaC.Store ℭ J
   init inputs := {
     inputs
     revision := 0
